src/ListLemmas.v
@@ -1,0 +1,77 @@
+(* Boring stuff, including but not limited to list lemmas *)
+Require Import Arith List Omega StructTact.StructTactics StuartTact.
+Import ListNotations.
+
+Require Import Monads.
+
+
+Lemma nat_max_le : forall n1 n2 m,
+    max n1 n2 <= m ->
+    n1 <= m /\ n2 <= m.
+intros0 Hle. destruct (Max.max_spec n1 n2) as [[? ?] | [? ?]]; split; omega.
+Qed.
+
+Lemma nat_max_le1 : forall n1 n2 m, max n1 n2 <= m -> n1 <= m.
+intros. destruct (nat_max_le ?? ?? ?? **). assumption.
+Qed.
+
+Lemma nat_max_le2 : forall n1 n2 m, max n1 n2 <= m -> n2 <= m.
+intros. destruct (nat_max_le ?? ?? ?? **). assumption.
+Qed.
+
+Lemma nat_le_max : forall n1 n2 m,
+    n1 <= m ->
+    n2 <= m ->
+    max n1 n2 <= m.
+intros0 Hle1 Hle2. destruct (Max.max_spec n1 n2) as [[? ?] | [? ?]]; omega.
+Qed.
+
+
+Fixpoint maximum ns :=
+    match ns with
+    | [] => 0
+    | n :: ns => max n (maximum ns)
+    end.
+
+Lemma maximum_le_Forall_fwd : forall ns m,
+    maximum ns <= m ->
+    Forall (fun n => n <= m) ns.
+induction ns; intros; simpl in *; eauto using nat_max_le1, nat_max_le2.
+Qed.
+
+Lemma maximum_le_Forall_rev : forall ns m,
+    Forall (fun n => n <= m) ns ->
+    maximum ns <= m.
+induction ns; inversion 1; [simpl; omega | eauto using nat_le_max].
+Qed.
+
+Lemma maximum_le_Forall : forall ns m,
+    maximum ns <= m <-> Forall (fun n => n <= m) ns.
+intros; split; eauto using maximum_le_Forall_fwd, maximum_le_Forall_rev.
+Qed.
+
+
+Fixpoint map_partial {A B : Type} (f : A -> option B) (l : list A) : option (list B) :=
+  match l with
+  | [] => Some []
+  | a :: l' => match f a, map_partial f l' with
+              | Some b, Some l'' => Some (b :: l'')
+              | _, _ => None
+              end
+  end.
+
+Lemma map_partial_Forall2 : forall A B (f : A -> option B) xs ys,
+    map_partial f xs = Some ys ->
+    Forall2 (fun x y => f x = Some y) xs ys.
+induction xs; intros0 Hmap; destruct ys; simpl in *; repeat break_match; try congruence.
+- constructor.
+- inject_some. specialize (IHxs _ ***). constructor; eauto.
+Qed.
+
+Lemma Forall2_map_partial : forall A B (f : A -> option B) xs ys,
+    Forall2 (fun x y => f x = Some y) xs ys ->
+    map_partial f xs = Some ys.
+induction xs; inversion 1; subst; simpl in *.
+- reflexivity.
+- find_rewrite. erewrite IHxs by eauto. reflexivity.
+Qed.
